minor documentation and alternate version of alloc added

Verse/Function.v
@@ -9,6 +9,15 @@ Require Import Basics.
 
 Set Implicit Arguments.
 
+(* Function record parametrized by the varT and type of the loopvar *)
+Record Function (v : varT) t    := func
+                                {
+                                  setup    : block v;
+                                  loop     : v t -> block v;
+                                  cleanup  : block v;
+                                }.
+
+(* Internal type which does not hide the loopvar from other blocks *)
 Record FB (v : varT) t := fb
                                 {
                                   pre    : block v;
@@ -17,36 +26,25 @@ Record FB (v : varT) t := fb
                                   post   : block v;
                                 }.
 
-Record Function (v : varT) t    := func
-                                {
-                                  setup    : block v;
-                                  loop     : v t -> block v;
-                                  cleanup  : block v;
-                                }.
-
+(* v l1 -> v l2 -> ... -> T *)
 Fixpoint lamT (v : varT) (l : list type) (T : Type) : Type :=
   match l with
   | [] => T
   | ty :: lt => v ty -> lamT v lt T
   end.
 
+(* Instantiation of a lamT *)
 Definition betaT v l := forall T, lamT v l T -> T.
 
+(* The user-defined function using the lamT to provide variables *)
 Definition function (p lv lr : list type) t :=
   forall (v : varT), lamT v (p ++ lv ++ lr) (Function v t).
 
-(*
-I could not write any of the below without proof mode. Have not taken time
-to make the proofs clean, concentrated on completion.
- *)
-
-
 (* A list-like constructor for betaT *)
-Definition beta_app v t (vt : v t) (l : list type) (b : betaT v l) : betaT v (t :: l).
+Lemma beta_app v t (vt : v t) (l : list type) (b : betaT v l) : betaT v (t :: l).
 unfold betaT. unfold lamT. fold lamT.
 exact (fun T f => b T (f vt)).
 Qed.
-
 
 (* lamT 'commutes' with ++ *)
 Lemma lamT_app : forall {v} {l1 l2} {T}, lamT v (l1 ++ l2) T = lamT v l1 (lamT v l2 T).
@@ -59,7 +57,7 @@ Proof.
   trivial.
 Qed.
 
-(* lamT is funco T *)
+(* lamT is functorial on T *)
 Definition lamFT {T T'} (f : T -> T') {v l} : (lamT v l T) -> (lamT v l T').
   induction l.
   eauto.
@@ -77,8 +75,8 @@ Proof.
   exact (IHl (X (f _ X0))).
 Qed.
 
-(* Best explained on call *)
-Definition tr' v l t : lamT v l (Function v t) -> lamT v ([t] ++ l) (FB v t).
+(* Constructs a parametrized FB from a parametrized Function *)
+Definition beta_loop v l t : lamT v l (Function v t) -> lamT v ([t] ++ l) (FB v t).
   intros.
   unfold lamT. simpl. fold lamT.
   induction l.
@@ -88,13 +86,19 @@ Definition tr' v l t : lamT v l (Function v t) -> lamT v ([t] ++ l) (FB v t).
   exact (fun x y => IHl (X y) x).
 Qed.
 
+(* 
+Breaks up the lamT parametrizing a Function into two lamT's which would be
+instantiated by callConv and lalloc respectively.
+This is with the assumption that the loopvar is allocated on the stack by the callConv.
+ *)
+
 Definition tr {p lv lr} t (f : function p lv lr t) : forall v, lamT v (p ++ lv ++ [t]) (lamT v lr (FB v t)).
   intros.
   unfold function in f.
   rewrite app_assoc in f.
   assert (f' := f v).
   rewrite lamT_app in f'.
-  assert (f'':= lamFT (tr' v lr t) f').
+  assert (f'':= lamFT (beta_loop v lr t) f').
   rewrite <- lamT_app in f''.
   rewrite app_assoc in f''.
   rewrite lamT_app in f''.
@@ -102,4 +106,17 @@ Definition tr {p lv lr} t (f : function p lv lr t) : forall v, lamT v (p ++ lv +
   exact f''.
 Qed.
 
+(*
+Does the same as above but with the assumption that loopvar is allocated on a register
+and by the user.
+*)
+
+Definition tr' {p lv lr} t (f : function p lv lr t) : forall v, lamT v (p ++ lv) (lamT v (t :: lr) (FB v t)).
+  intros.
+  unfold function in f.
+  rewrite app_assoc in f.
+  assert (f' := f v).
+  rewrite lamT_app in f'.
+  exact (lamFT (beta_loop v lr t) f').
+Qed.
 
